Checkpoint progress on double indirect blocks

src/Inode.v
@@ -108,6 +108,7 @@ Module INODE.
   Definition xp_to_raxp xp :=
     RecArray.Build_xparams (IXStart xp) (IXLen xp).
 
+
   (** `ilist` is a list of inodes *)
   Definition irrep xp (ilist : list irec) :=
     ([[ length ilist = wordToNat (IXLen xp ^* items_per_valu) ]] *
@@ -239,8 +240,6 @@ Module INODE.
     reflexivity.
   Qed.
 
-
-
   Theorem indirect_bound : forall Fm bxp bn l m,
     (Fm * indrep bxp bn l)%pred m -> length l <= wordToNat wnr_indirect.
   Proof.
@@ -330,9 +329,242 @@ Module INODE.
   Definition dindxp bn := RecArray.Build_xparams bn $1.
 
   (** The block at `bn` is a doubly indirect block that contains a list of addresses of indirect blocks *)
-  Definition dindrep bxp bn (blist : list addr) :=
-    ([[ length blist = nr_ind_in_dindirect ]] * [[ BALLOC.valid_block bxp bn ]] *
-     RecArray.array_item dindtype wnr_ind_in_dindirect dindsz_ok (dindxp bn) blist)%pred.
+  Definition dindrep bxp bn (indlist : list addr) :=
+    ([[ length indlist = nr_ind_in_dindirect ]] * [[ BALLOC.valid_block bxp bn ]] *
+     RecArray.array_item dindtype wnr_ind_in_dindirect dindsz_ok (dindxp bn) indlist)%pred.
+
+(*
+  Definition dindrep2 bxp bn off indlist  :=
+    (exists indlist indaddr ind_ v,
+    [[ length  = nr_dindirect ]] * 
+    [[ (off |-> v) (list2mem ) ]] *
+    dindrep bxp bn indlist *
+    [[ ((off ^/ wnr_ind_in_dindirect) |-> indaddr) (list2mem indlist) ]] *
+    indrep bxp indaddr ind_ *
+    [[ ((off ^% wnr_ind_in_dindirect) |-> v) (list2mem ind_) ]])%pred.
+*)
+Print Forall.
+Print In.
+
+Print seq.
+  Definition dindrep_big bxp bn indlist (blist : list addr) :=
+    (exists indblocks, dindrep bxp bn indlist
+      * listmatch (indrep bxp) indlist indblocks
+      * [[ length blist = nr_dindirect ]]
+      * [[ blist = concat indblocks ]]
+      )%pred.
+
+  Definition sublist (A:Type) (n m:nat) (l:list A) :=
+    skipn n (firstn m l).
+
+  Theorem dindrep_big_seq : forall A B bxp bn indlist blist off v v2 m,
+    (dindrep_big bxp bn indlist blist * [[ off < nr_dindirect ]]
+      * exists indblks, indrep bxp v2 indblks
+      * [[(A * (off mod nr_ind_in_dindirect) |-> v)%pred (list2nmem indblks) ]]
+      * [[(B * (off / nr_ind_in_dindirect) |-> v2)%pred (list2nmem indlist) ]])%pred m ->
+      selN blist off $0 = v.
+  Proof.
+    unfold dindrep_big, indrep.
+    intros. destruct_lift H.
+    unfold dindrep, listmatch in H.
+    destruct_lift H.
+    admit.
+  Admitted.
+
+  Definition blist_ind (blist : list addr) off :=
+    let start := ((off ^/ wnr_ind_in_dindirect) ^* wnr_ind_in_dindirect) in
+    sublist (# start) ((# start) + nr_ind_in_dindirect) blist.
+
+  Theorem map_skip_comm : forall T V (l : list T) (f : T -> V) n, skipn n (map f l) = map f (skipn n l).
+  Proof.
+    intros. generalize dependent l.
+    induction n; auto.
+    induction l; auto.
+    simpl. rewrite IHn. reflexivity.
+  Qed.
+  Theorem map_sublist_comm : forall T V (l : list T) (f : T -> V) m n, map f (sublist m n l) = sublist m n (map f l).
+  Proof.
+    unfold sublist.
+    intros. erewrite LOG.firstn_map.
+    rewrite map_skip_comm. auto.
+  Qed.
+
+  Theorem selN_skipn : forall T (l : list T) n i, selN (skipn n l) i = selN l (n + i).
+  Proof.
+    intros. generalize dependent l. induction n; auto.
+    intros. simpl. induction l; auto; simpl in *. rewrite IHn; try omega. unfold selN. reflexivity.
+  Qed.
+  Fact off_div_wnr_indirect_lt_addrlen_N : forall (off : addr), #(off) < nr_dindirect ->
+    (N.of_nat # (off) / N.of_nat # (wnr_indirect) < Npow2 addrlen)%N.
+  Proof. intros.
+    apply N.div_lt_upper_bound.
+    compute. intuition. inversion H0.
+    rewrite wordToNat_wnr_indirect.
+
+    apply Nomega.Nlt_in.
+    rewrite N2Nat.inj_mul.
+    repeat rewrite N2Nat.id;
+    repeat rewrite Nat2N.id.
+    eapply Nat.lt_trans.
+    apply H.
+    unfold nr_dindirect.
+    Search (_ * _ < _).
+    apply mult_lt_compat_l.
+    rewrite <- Nat2N.id with (n := nr_ind_in_dindirect).
+    apply Nomega.Nlt_out. compute. auto. compute. omega.
+  Qed.
+
+
+  Theorem sublist_blist : forall off blist a v, length blist = nr_dindirect ->
+    v = selN blist #off a ->  #off < length blist ->
+    (selN (blist_ind blist off) (#(off ^% wnr_ind_in_dindirect)) a) = v.
+  Proof. intros.
+
+    unfold blist_ind, sublist.
+    rewrite selN_skipn. rewrite wnr_in_dindirect_eq_wnr_indirect.
+    rewrite selN_firstn.
+    Search wordToNat.
+    unfold wdiv, wmult, wmod.
+    unfold wordBin.
+    repeat rewrite wordToN_nat.
+    rewrite N.mul_comm.
+    Search NToWord.
+    repeat rewrite N2Nat_word.
+    Search N.div.
+    Search N.of_nat.
+    rewrite Ninj_mod.
+    rewrite Ninj_div.
+    rewrite N2Nat.inj_mul.
+    Search N.to_nat.
+    repeat rewrite N2Nat.id.
+    repeat rewrite Nat2N.id.
+    Search (_ * (_ / _ ) ).
+    rewrite <- Nat.div_mod.
+    symmetry. assumption.
+
+    compute; intuition.
+    compute; intuition.
+    eapply N.lt_trans.
+    Search N.modulo.
+    apply N.mod_lt.
+    compute; intuition; inversion H2.
+    compute; auto.
+    Search N.div.
+    apply off_div_wnr_indirect_lt_addrlen_N; omega.
+    rewrite <- Nat2N.inj_mul.
+    rewrite Ninj_div.
+    apply Nomega.Nlt_in.
+    repeat rewrite Nat2N.id; repeat rewrite N2Nat.id. rewrite wordToNat_wnr_indirect.
+    Search ( _ * (_ / _ )).
+    assert (nr_indirect * (# (off) / nr_indirect) <= # off).
+    Search (_ <= _).
+    apply Nat.mul_div_le; compute; intuition.
+    Search (_ <= _ -> _ < _).
+    eapply Nat.le_lt_trans. apply H2.
+    rewrite H in H1. eapply lt_trans. apply H1.
+    Search (_ < _ -> (_ < _)).
+    Search nr_dindirect.
+    SearchAbout nr_dindirect.
+    admit.
+    apply off_div_wnr_indirect_lt_addrlen_N.
+    omega.
+    Search (_ +_ < _ + _).
+    apply plus_lt_compat_l.
+    Search nr_indirect.
+    rewrite nr_in_dindirect_eq_nr_indirect.
+    unfold wnr_indirect.
+    apply lt_word_lt_nat.
+    unfold wmod, wordBin.
+    apply Nomega.Nlt_in.
+    repeat rewrite wordToN_nat.
+    repeat rewrite N2Nat_word.
+    rewrite Ninj_mod.
+    repeat rewrite N2Nat.id;
+    repeat rewrite Nat2N.id.
+    Search Nat.modulo.
+    apply Nat.mod_bound_pos. omega. compute. omega. compute. intuition.
+    admit.
+  Admitted.
+
+(*
+  Fix group A (l : list A) (s : list A) (n : nat) (k : nat) : list (list A) :=
+    match l with
+    | nil => [ [] ]
+    | x :: l' => 
+      match k with
+      | n => group A l' [x] n 0
+      | else => 
+*)
+    Theorem concat_eq_nil : forall T (l : list (list T)), concat l = [] -> Forall (eq []) l.
+    Proof.
+      intros. induction l; eauto. destruct a; eauto. simpl in H. inversion H.
+    Qed.
+
+    Theorem concat_repeat_nil : forall A n, @concat A (repeat [] n) = [].
+    Proof. induction n; eauto.
+    Qed.
+
+    Theorem concat_eq_nil_eq_repeat : forall T (l : list (list T)) n, concat l = [] -> length l = n -> l = repeat [] n.
+    Proof.
+      intros. subst. apply concat_eq_nil in H.
+      induction l; auto.
+      inversion H. subst. simpl. rewrite <- IHl; auto.
+    Qed.
+
+(*
+  Theorem dindrep_big_split_length : forall m bxp bn indlist ,
+    (dindrep_big bxp bn indlist ) m ->
+    (ngth  = nr_dindirect).
+  Proof.
+    intros. unfold dindrep_big in H. destruct_lift H.
+    Search (_ /\ _). assumption.
+  Qed.
+
+Search Forall.
+*)
+(*
+  Definition dindrep_total bxp bn ( : list addr) :=
+    (exists indlist indaddr,
+      (dindrep bxp bn bn_indlist)
+     [[ (ind |-> indaddr)%pred (list2mem bn_indlist) ]]
+     * (indrep bxp indaddr indlist)
+     * [[ (ind_off |-> baddr)%pred (list2mem indlist) ]]
+     * [[ (off |-> baddr) (list2mem ) ]]
+     * [[ ((ind ^* wnr_ind_in_dindirect ^+ ind_off) |-> baddr)%pred (list2mem ) ]])%pred.
+*)
+(*
+  Definition dindrep_again bxp bn ( : list addr) :=
+    (exists bn_indlist ind indaddr indlist baddr, (dindrep bxp bn bn_indlist)
+     * [[ (ind |-> indaddr)%pred (list2mem bn_indlist) ]]
+     * (indrep bxp indaddr indlist)
+     * [[ (ind_off |-> baddr)%pred (list2mem indlist) ]]
+     * [[ (off |-> baddr) (list2mem ) ]]
+     * [[ ((ind ^* wnr_ind_in_dindirect ^+ ind_off) |-> baddr)%pred (list2mem ) ]])%pred.
+*)
+Opaque nr_ind_in_dindirect.
+(* 
+  Theorem dindrep_down : forall F G bxp dindaddr indlist  indindex indaddr indblocks index v0 m,
+    (dindrep_big bxp dindaddr indlist ) m ->
+    (F * indindex |-> indaddr)%pred (list2nmem indlist) ->
+    (indrep bxp indaddr indblocks) m ->
+    (G * index |-> v0)%pred (list2nmem indblocks) ->
+    (((index + nr_ind_in_dindirect * indindex) |-> v0)%pred (list2nmem )).
+  Proof.
+    intros.
+    unfold dindrep_big in H.
+    apply dindrep_big_split in 
+    Print pred_apply.
+    apply dindrep_big_split in H.
+    unfold dindrep_big in H. destruct_lift H.
+    SearchAbout list2nmem.
+    eapply list2nmem_sel in H0.
+    eapply list2nmem_sel in H2.
+    unfold indrep in H1. destruct_lift H1.
+    unfold indrep in H.
+    Search concat.
+
+
+    destruct_lift H. *)
 
   Definition dindget T lxp a off mscs rx : prog T :=
     let^ (mscs, v) <- RecArray.get dindtype wnr_ind_in_dindirect dindsz_ok
@@ -348,7 +580,7 @@ Module INODE.
     (Fm * dindrep bxp bn l)%pred m -> length l = nr_ind_in_dindirect.
   Proof.
     unfold dindrep; intros.
-    destruct_lift H; auto.
+    destruct_lift H. auto.
   Qed.
 
   Theorem wordToNat_wnr_ind_in_dindirect : # wnr_ind_in_dindirect = nr_ind_in_dindirect.
@@ -378,23 +610,29 @@ Module INODE.
     unfold dindget, dindrep, dindxp.
     hoare.
   Qed.
-
-  Definition dindrep_internal bxp blist indlist :=
-    (exists ind_block, [[ blist = concat ind_block ]] *
-     listmatch (fun indaddr contents => indrep bxp indaddr contents) indlist ind_block)%pred.
-
-  Definition n_dindirect := N.of_nat nr_dindirect.
-
-  Theorem n_dindirect_eqiv_nr_dindirect : nr_dindirect = N.to_nat n_dindirect.
+(*
+  Theorem dindget_ok' : forall lxp bxp a off mscs,
+    {< F Fm A B C mbase m indlist blist indaddr indblks v,
+    PRE          LOG.rep lxp F (ActiveTxn mbase m) mscs *
+                  [[ (Fm * dindrep bxp a indlist)%pred (list2mem m) ]] *
+                  [[ (A * #(off ^/ wnr_ind_in_dindirect) |-> indaddr )%pred (list2nmem indlist) ]] *
+                  [[ (Fm * indrep bxp a indblks)%pred (list2mem m) ]] *
+                  [[ (B * #(off ^% wnr_ind_in_dindirect) |-> v )%pred (list2nmem indblks) ]] *
+                  [[ (C * #(off) |-> v)%pred (list2nmem blist) ]]
+    POST RET:^(mscs,r)
+                  LOG.rep lxp F (ActiveTxn mbase m) mscs *
+                  [[ (A * #(off ^/ wnr_ind_in_dindirect) |-> indaddr )%pred (list2nmem indlist) ]] *
+                  [[ (Fm * indrep bxp a indblks)%pred (list2mem m) ]] *
+                  [[ (B * #(off ^% wnr_ind_in_dindirect) |-> v )%pred (list2nmem indblks) ]] *
+                  [[ (C * #(off) |-> v)%pred (list2nmem blist) ]] *
+                  [[ r = indaddr ]]
+    CRASH         LOG.would_recover_old lxp F mbase
+    >} dindget lxp a off mscs.
   Proof.
-    unfold n_dindirect. rewrite Nat2N.id. auto.
+    unfold dindget, dindrep, dindxp.
+    hoare.
   Qed.
-
-  Theorem n_dindirect_eqiv_nr_dindirect' : n_dindirect = N.of_nat nr_dindirect.
-  Proof.
-    unfold n_dindirect. reflexivity.
-  Qed.
-
+*)
   Theorem dindput_ok : forall lxp bxp a off bn mscs,
     {< F Fm A mbase m indlist v0,
     PRE       LOG.rep lxp F (ActiveTxn mbase m) mscs *
@@ -441,6 +679,51 @@ Module INODE.
   Local Hint Resolve wle_le.
   Hint Rewrite removeN_updN : core.
 
+  Definition indlist0 := repeat (natToWord inditemsz 0) nr_indirect.
+
+  Theorem ind_ptsto : forall bxp a vs,
+    indrep bxp a vs
+    =p=> (a |-> (rep_block indsz_ok vs))%pred.
+  Proof.
+    unfold indrep, array_item, array_item_pairs, indxp.
+    cancel.
+    destruct vs_nested; inversion H0.
+    pose proof (length_nil vs_nested) as Hx.
+    apply Hx in H4; subst; simpl in *.
+    rewrite app_nil_r; subst.
+    cancel.
+  Qed.
+
+Opaque wnr_indirect.
+
+  Theorem ind_ptsto_zero : forall a,
+    (a |-> $0)%pred =p=>
+    array_item indtype wnr_indirect indsz_ok (indxp a) indlist0.
+  Proof.
+    intros.
+    unfold array_item, array_item_pairs, indxp.
+    norm.
+    instantiate (vs_nested := [ RecArray.block_zero indtype wnr_indirect ]).
+    unfold rep_block, block_zero, wreclen_to_valu; simpl.
+    rewrite Rec.to_of_id.
+    rewrite indsz_ok; auto.
+
+    unfold block_zero.
+    rewrite wordToNat_wnr_indirect. unfold nr_indirect.
+    rewrite Forall_forall.
+    intuition.
+    simpl in H; intuition; subst; auto.
+    rewrite Forall_forall; auto.
+  Qed.
+
+
+  Theorem indlist0_length : length indlist0 = nr_indirect.
+  Proof.
+    unfold indlist0; apply repeat_length.
+  Qed.
+
+  Local Hint Resolve indlist0_length.
+
   Definition dindlist0 := repeat (natToWord dinditemsz 0) nr_ind_in_dindirect.
 
   Theorem dind_ptsto : forall bxp a vs,
@@ -456,7 +739,6 @@ Module INODE.
     apply Hx in H4. subst. simpl in *.
     rewrite app_nil_r. cancel.
   Qed.
-
 
   Theorem dind_ptsto_zero : forall a,
     (a |-> $0)%pred =p=>
@@ -482,50 +764,7 @@ Module INODE.
     unfold dindlist0; apply repeat_length.
   Qed.
 
-
   Local Hint Resolve dindlist0_length.
-
-  Definition indlist0 := repeat (natToWord inditemsz 0) nr_indirect.
-
-  Theorem ind_ptsto : forall bxp a vs,
-    indrep bxp a vs
-    =p=> (a |-> (rep_block indsz_ok vs))%pred.
-  Proof.
-    unfold indrep, array_item, array_item_pairs, indxp.
-    cancel.
-    destruct vs_nested; inversion H0.
-    pose proof (length_nil vs_nested) as Hx.
-    apply Hx in H4; subst; simpl in *.
-    rewrite app_nil_r; subst.
-    cancel.
-  Qed.
-
-  Theorem ind_ptsto_zero : forall a,
-    (a |-> $0)%pred =p=>
-    array_item indtype wnr_indirect indsz_ok (indxp a) indlist0.
-  Proof.
-    intros.
-    unfold array_item, array_item_pairs, indxp.
-    norm.
-    instantiate (vs_nested := [ RecArray.block_zero indtype wnr_indirect ]).
-    unfold rep_block, block_zero, wreclen_to_valu; simpl.
-    rewrite Rec.to_of_id.
-    rewrite indsz_ok; auto.
-
-    unfold block_zero.
-    rewrite Forall_forall.
-    intuition.
-    simpl in H; intuition; subst; auto.
-    rewrite Forall_forall; auto.
-  Qed.
-
-
-  Theorem indlist0_length : length indlist0 = nr_indirect.
-  Proof.
-    unfold indlist0; apply repeat_length.
-  Qed.
-
-  Local Hint Resolve indlist0_length.
 
   (* separation logic based theorems *)
 
@@ -758,29 +997,30 @@ Module INODE.
     simpl. omega.
   Qed.
 
-  Definition dindirect_valid bxp n bn blist :=
-     ([[ n <= nr_direct + nr_indirect ]] \/ [[ n > nr_direct + nr_indirect]] * dindrep bxp bn blist)%pred.
 
-  Lemma dindirect_valid_r : forall bxp n bn blist,
+  Definition dindirect_valid bxp n bn indlist :=
+     ([[ n <= nr_direct + nr_indirect ]] \/ [[ n > nr_direct + nr_indirect]] * dindrep bxp bn indlist)%pred.
+
+  Lemma dindirect_valid_r : forall bxp n bn indlist,
     n > nr_direct + nr_indirect
-    -> dindirect_valid bxp n bn blist <=p=> dindrep bxp bn blist.
+    -> dindirect_valid bxp n bn indlist <=p=> dindrep bxp bn indlist.
   Proof.
     intros. unfold dindirect_valid, piff; split; cancel.
     omega.
   Qed.
 
-  Lemma dindirect_valid_l : forall bxp n bn blist,
+  Lemma dindirect_valid_l : forall bxp n bn indlist,
     n <= nr_direct + nr_indirect
-    -> dindirect_valid bxp n bn blist <=p=> emp.
+    -> dindirect_valid bxp n bn indlist <=p=> emp.
   Proof.
     intros. unfold dindirect_valid, piff; split; cancel.
     omega.
   Qed.
 
-  Lemma dindirect_valid_r_off : forall bxp n off bn blist,
+  Lemma dindirect_valid_r_off : forall bxp n off bn indlist,
     wordToNat off < n
     -> (off >= wnr_direct ^+ wnr_indirect)%word
-    -> dindirect_valid bxp n bn blist <=p=> dindrep bxp bn blist.
+    -> dindirect_valid bxp n bn indlist <=p=> dindrep bxp bn indlist.
   Proof.
     auto; intros.
     apply dindirect_valid_r.
@@ -789,39 +1029,45 @@ Module INODE.
     omega.
   Qed.
 
-  Definition dindirect_internal_valid bxp n blist indlist:=
-     ([[ n <= nr_direct + nr_indirect ]] \/ [[ n > nr_direct + nr_indirect]] * dindrep_internal bxp blist indlist)%pred.
+  Print dindrep_again.
 
-  Lemma dindirect_internal_valid_r : forall bxp n blist indlist,
+  Definition dindirect_internal_valid bxp n bn off blist ind indaddr off baddr :=
+     ([[ n <= nr_direct + nr_indirect ]] \/ 
+      [[ n > nr_direct + nr_indirect]] * 
+      dindrep_again bxp bn bn_indlist indlist blist ind indaddr off baddr)%pred.
+
+  Lemma dindirect_internal_valid_r : forall bxp n bn bn_indlist indlist blist ind indaddr off baddr,
     n > nr_direct + nr_indirect
-    -> dindirect_internal_valid bxp n blist indlist <=p=> dindrep_internal bxp blist indlist.
+    -> dindirect_internal_valid bxp n bn bn_indlist indlist blist ind indaddr off baddr
+        <=p=> dindrep_again bxp bn bn_indlist indlist blist ind indaddr off baddr.
   Proof.
     intros. unfold dindirect_internal_valid, piff; split; cancel.
     omega.
   Qed.
 
-  Lemma dindirect_internal_valid_l : forall bxp n blist indlist,
+  Lemma dindirect_internal_valid_l : forall bxp n bn bn_indlist indlist blist ind indaddr off baddr,
     n <= nr_direct + nr_indirect
-    -> dindirect_internal_valid bxp n blist indlist <=p=> emp.
+    -> dindirect_internal_valid bxp n bn bn_indlist indlist blist ind indaddr off baddr
+        <=p=> emp.
   Proof.
     intros. unfold dindirect_internal_valid, piff; split; cancel.
     omega.
   Qed.
 
-  Lemma dindirect_internal_valid_r_off : forall bxp n off blist indlist,
+  Fact wordToNat_wnr_direct_plus_wnr_indirect : # (wnr_direct ^+ wnr_indirect) = nr_direct + nr_indirect.
+  Proof. auto. Qed.
+
+  Lemma dindirect_internal_valid_r_off : forall bxp n (off : nat) bn bn_indlist indlist blist ind indaddr off baddr,
     wordToNat off < n
     -> (off >= wnr_direct ^+ wnr_indirect)%word
-    -> dindirect_internal_valid bxp n blist indlist <=p=> dindrep_internal bxp blist indlist.
+    -> dindirect_internal_valid bxp n bn bn_indlist indlist blist ind indaddr off baddr
+        <=p=> dindrep_again bxp bn bn_indlist indlist blist ind indaddr off baddr.
   Proof.
     auto; intros.
     apply dindirect_internal_valid_r.
-    apply wle_le in H0.
-    replace (wordToNat (wnr_direct ^+ wnr_indirect)) with (nr_direct + nr_indirect) in * by auto.
+    apply wle_le in H0. Search (wnr_direct ^+ wnr_indirect).
+    rewrite wordToNat_wnr_direct_plus_wnr_indirect in H0.
     omega.
-  Qed.
-
-  Lemma wnr_direct_plus_indirect_ok : # (wnr_direct ^+ wnr_indirect) = nr_direct + nr_indirect.
-    reflexivity.
   Qed.
 
   (** The inode `ino` is equivalent to the on-disk record `rec` *)
@@ -830,8 +1076,7 @@ Module INODE.
     [[ length (IBlocks ino) <= blocks_per_inode ]] *
     [[ iattr_match (IAttr ino) (rec :-> "attr") ]] *
     exists indlist, indirect_valid bxp (length (IBlocks ino)) (rec :-> "indptr") indlist *
-    exists dind_indlist, dindirect_valid bxp (length (IBlocks ino)) (rec :-> "dindptr") dind_indlist *
-    exists dindlist, dindirect_internal_valid bxp (length (IBlocks ino)) dindlist dind_indlist *
+    exists dindlist, dindirect_total_valid bxp (length (IBlocks ino)) (rec :-> "dindptr") dindlist *
     [[ IBlocks ino = firstn (length (IBlocks ino)) ((rec :-> "blocks") ++ indlist ++ dindlist) ]]
     )%pred.
 
@@ -901,8 +1146,6 @@ Module INODE.
   Qed.
 
   Arguments Rec.well_formed : simpl never.
-
-
 
   Lemma wle_eq_le: forall sz (a : word sz) b c,
     b <= wordToNat (natToWord sz b)
@@ -1001,7 +1244,6 @@ Module INODE.
   Hint Rewrite resolve_selN_addr0   using reflexivity : defaults.
   Hint Rewrite resolve_sel_valu0    using reflexivity : defaults.
   Hint Rewrite resolve_selN_valu0   using reflexivity : defaults.
-
 
   Lemma rep_bound: forall Fm bxp xp l m,
     (Fm * rep bxp xp l)%pred m
@@ -1199,6 +1441,13 @@ Module INODE.
     >} iget lxp xp inum off mscs.
   Proof.
     unfold iget, rep.
+    hoare.
+    admit.
+    
+    Search listmatch.
+
+
+
     step.
     list2nmem_ptsto_cancel; inode_bounds.
 
@@ -1208,8 +1457,7 @@ Module INODE.
     (* from direct blocks *)
     repeat rewrite_list2nmem_pred.
     destruct_listmatch_n.
-    unfold sel; subst.
-    rewrite H19.
+    rewrite H21.
     rewrite selN_firstn by inode_bounds.
     rewrite selN_app; [ inode_bounds |].
     erewrite inode_blocks_length with (m := list2mem m); inode_bounds.
@@ -1219,12 +1467,13 @@ Module INODE.
     (* from indirect blocks *)
     repeat rewrite_list2nmem_pred.
     destruct_listmatch_n.
-    step.
-
+    step. step.
     erewrite indirect_valid_r_off; eauto.
-    list2nmem_ptsto_cancel; inode_bounds.
+    cancel. 
+    list2nmem_ptsto_cancel.
+    Search dummy0.
     eapply indirect_valid_off_bound; eauto.
-
+    erewrite indirect_valid_r_off; eauto.
     step.
     subst.
     rewrite H19.
@@ -1601,6 +1850,28 @@ Module INODE.
     exact $0.
     exact emp.
   Qed.
+
+
+  Theorem igrow_dindirect_ok : forall lxp bxp xp (i0 : irec) inum a mscs,
+    {< F Fm A B mbase m ilist (reclist : list irec) ino,
+    PRE      LOG.rep lxp F (ActiveTxn mbase m) mscs *
+             [[ length (IBlocks ino) < blocks_per_inode ]] *
+             [[ i0 :-> "len" > wnr_direct + wnr_indirect ]]%word *
+             [[ i0 = sel reclist inum irec0 ]] *
+             [[ (Fm * irrep xp reclist *
+                 listmatch (inode_match bxp) ilist reclist)%pred (list2mem m) ]] *
+             [[ (A * #inum |-> ino)%pred (list2nmem ilist) ]] *
+             [[  B (list2nmem (IBlocks ino)) ]]
+    POST RET:^(mscs,r)
+             exists m' ilist' ino',
+             LOG.rep lxp F (ActiveTxn mbase m') mscs *
+             [[ r = true ]] *
+             [[ (Fm * rep bxp xp ilist')%pred (list2mem m') ]] *
+             [[ (A * #inum |-> ino')%pred (list2nmem ilist') ]] *
+             [[ (B * length (IBlocks ino) |-> a)%pred (list2nmem (IBlocks ino')) ]] *
+             [[ ino' = Build_inode ((IBlocks ino) ++ [a]) (IAttr ino) ]]
+    CRASH    LOG.would_recover_old lxp F mbase
+    >} igrow_dindirect lxp bxp xp i0 inum a mscs.
 
 
   Hint Extern 1 ({{_}} progseq (igrow_direct _ _ _ _ _ _) _) => apply igrow_direct_ok : prog.
